RGA last proof-direct

inductive_proof/RGA_set_pre-cond/App_do_pre_first.fst
@@ -54,34 +54,28 @@ let get_after_id (op:op_t{Add_after? (snd op)}) : nat =
 let get_rem_id (op:op_t{Remove? (snd op)}) : pos =
   let (_, Remove id) = op in id
 
-(*let do_pre (s:concrete_st) (op:op_t) : prop =
-  match op with
-  |(ts, Add_after after_id ele) -> ~ (mem_id_s ts (fst s)) /\                            
-                                  (~ (after_id = 0) ==> mem_id_s after_id (fst s))
-  |(_, Remove id) -> mem_id_s id (fst s) /\ ~ (S.mem id (snd s))*)
-  
 let do_pre (s:concrete_st) (op:op_t) : prop =
   match op with
-  |(ts, Add_after after_id ele) -> ~ (mem_id_s ts (fst s))                               
-                                  //(~ (after_id = 0) ==> mem_id_s after_id (fst s))
-  |(ts, Remove id) -> True //mem_id_s id (fst s) /\ ~ (S.mem id (snd s))
+  |(ts, Add_after after_id ele) -> ~ (mem_id_s ts (fst s)) /\ //after_id <> ts /\                            
+                                  (~ (after_id = 0) ==> mem_id_s after_id (fst s))
+  |(_, Remove id) -> mem_id_s id (fst s) /\ mem_id_s id (fst s)  ///\ ~ (S.mem id (snd s))
+
+let do_prop (s:concrete_st) (op:op_t) :
+  Lemma (ensures (Add_after? (snd op) ==> (do_pre s op <==>
+                           ~ (mem_id_s (fst op) (fst s)))) /\ //get_after_id op <> fst op /\                          
+                                  //(~ ((get_after_id op) = 0) ==> mem_id_s (get_after_id op) (fst s)))) /\
+                 (Remove? (snd op) ==> (do_pre s op <==>
+                          mem_id_s (get_rem_id op) (fst s)))) = ()
 
 // apply an operation to a state
-(*let do (s:concrete_st) (op:op_t{do_pre s op}) 
-  : (r:concrete_st{(Add_after? (snd op) ==> (forall id. mem_id_s id (fst r) <==> mem_id_s id (fst s) \/ id = fst op)) /\
-                   (Remove? (snd op) ==> (forall id. S.mem id (snd r) <==> S.mem id (snd s) \/ id = get_rem_id op)) /\
-                   S.subset (fst s) (fst r) /\ S.subset (snd s) (snd r)}) =
+let do (s:concrete_st) (op:op_t{do_pre s op}) 
+  : (r:concrete_st{(*//(Add_after? (snd op) ==> (forall id. mem_id_s id (fst r) <==> mem_id_s id (fst s) \/ id = fst op)) /\
+                   //(Remove? (snd op) ==> (forall id. S.mem id (snd r) <==> S.mem id (snd s) \/ id = get_rem_id op)) /\*)
+                    S.subset (fst s) (fst r) /\ S.subset (snd s) (snd r)}) =
    match op with
-  |(ts, Add_after after_id ele) -> (S.add (ts, (after_id, ele)) (fst s), snd s)
-  |(_, Remove id) -> (fst s, S.add id (snd s))*)
-  
-let do (s:concrete_st) (op:op_t{do_pre s op}) : (r:concrete_st{S.subset (fst s) (fst r) /\ S.subset (snd s) (snd r)}) =  
- 
-  match op with
-  |(ts, Add_after after_id ele) -> if (after_id <> 0 && not (mem_id_s after_id (fst s))) then s 
-                                  else (S.add (ts, (after_id, ele)) (fst s), snd s)
-  
-  |(_, Remove id) -> if mem_id_s id (fst s) (*&& not (S.mem id (snd s))*) then (fst s, S.add id (snd s)) else s
+  |(ts, Add_after after_id ele) -> //if after_id <> 0 && not (mem_id_s after_id (fst s)) then s else
+                                   (S.add (ts, (after_id, ele)) (fst s), snd s)
+  |(_, Remove id) -> (fst s, S.add id (snd s))
   
 let lem_do (a b:concrete_st) (op:op_t)
    : Lemma (requires eq a b /\ do_pre a op)
@@ -112,20 +106,13 @@ let resolve_conflict_prop (x:op_t) (y:op_t{fst x <> fst y})
 
 // concrete merge pre-condition
 let merge_pre l a b =
-  //S.subset (fst l) (fst a) /\ S.subset (fst l) (fst b) /\
-  //S.subset (snd l) (snd a) /\ S.subset (snd l) (snd b) /\
+  S.subset (fst l) (fst a) /\ S.subset (fst l) (fst b) /\
+  S.subset (snd l) (snd a) /\ S.subset (snd l) (snd b) /\
   (forall id. mem_id_s id (fst l) ==> ~ (mem_id_s id (S.difference (fst a) (fst l)))) /\
   (forall id. mem_id_s id (fst l) ==> ~ (mem_id_s id (S.difference (fst b) (fst l)))) /\
   (forall id. mem_id_s id (S.difference (fst a) (fst l)) ==> ~ (mem_id_s id (S.difference (fst b) (fst l))))
 
 let concrete_merge (lca s1:concrete_st) (s2:concrete_st{merge_pre lca s1 s2}) : concrete_st =
-  (*(S.union (S.intersect (fst lca) (S.intersect (fst s1) (fst s2))) 
-           (S.union (S.difference (fst s1) (fst lca)) (S.difference (fst s2) (fst lca))),
-   S.union (snd lca) (S.union (snd s1) (snd s2)))*)
-  
-   (*S.union (fst lca)
-           (S.union (S.difference (fst s1) (fst lca)) (S.difference (fst s2) (fst lca))),*)
-   
    (S.union (fst lca) (S.union (fst s1) (fst s2)),   
     S.union (snd lca) (S.union (snd s1) (snd s2)))
   
@@ -136,360 +123,163 @@ let merge_is_comm (lca s1 s2:st)
           (ensures merge_pre (v_of lca) (v_of s2) (v_of s1) /\
                    (eq (concrete_merge (v_of lca) (v_of s1) (v_of s2)) 
                        (concrete_merge (v_of lca) (v_of s2) (v_of s1)))) = ()           
-                      
-let linearizable_s1_0''_base_base (lca s1 s2':st) (last2:op_t)
-  : Lemma (requires do_pre (v_of s2') last2 /\
-                    consistent_branches lca s1 (do_st s2' last2) /\
-                    ops_of s1 = ops_of lca /\ ops_of s2' = ops_of lca /\
-                    length (ops_of lca) = 0 /\
-                    merge_pre (v_of lca) (v_of s1) (do (v_of s2') last2))
-        
-          (ensures eq (do (v_of s2') last2) (concrete_merge (v_of lca) (v_of s1) (do (v_of s2') last2))) = ()
 
-#push-options "--z3rlimit 100"
-let linearizable_s1_0''_do_pre (lca s1 s2':st) (last2:op_t)
-  : Lemma (requires do_pre (v_of s2') last2 /\
-                    consistent_branches lca s1 (do_st s2' last2) /\
-                    is_prefix (ops_of lca) (ops_of s2') /\
-                    ops_of s1 = ops_of lca /\                    
-                    fst last2 > 0 /\
-                    length (ops_of s2') > 0)
-         
-          (ensures do_pre (v_of (inverse_st s2')) last2) = ()
-
-let linearizable_s1_0''_base_merge_pre (lca s1 s2':st) (last2:op_t)
-  : Lemma (requires do_pre (v_of s2') last2 /\ 
-                    consistent_branches lca s1 (do_st s2' last2) /\
-                    ops_of s1 == ops_of lca /\ ops_of s2' == ops_of lca /\
-                    fst last2 > 0 /\
-                    merge_pre (v_of lca) (v_of s1) (do (v_of s2') last2) /\
-                    length (ops_of s2') > 0 /\
-                    do_pre (v_of (inverse_st s2')) last2)
-
-          (ensures (let l' = inverse_st lca in
-                    merge_pre (v_of l') (v_of l') (do (v_of l') last2))) = ()
-
-let linearizable_s1_0''_base_ind (lca s1 s2':st) (last2:op_t)
-  : Lemma (requires do_pre (v_of s2') last2 /\
-                    consistent_branches lca s1 (do_st s2' last2) /\
-                    ops_of s1 = ops_of lca /\ ops_of s2' = ops_of lca /\
-                    length (ops_of lca) > 0 /\
-
-                    (let l' = inverse_st lca in
-                    let s1' = inverse_st s1 in
-                    let s2'' = inverse_st s2' in
-                    do_pre (v_of s2'') last2 /\ 
-                    consistent_branches l' s1' (do_st s2'' last2) /\
-                    ops_of s1' = ops_of l' /\ ops_of s2'' = ops_of l' /\
-                    merge_pre (v_of l') (v_of s1') (do (v_of s2'') last2) /\
-                    eq (do (v_of s2'') last2) (concrete_merge (v_of l') (v_of s1') (do (v_of s2'') last2))) /\
-                    merge_pre (v_of lca) (v_of s1) (do (v_of s2') last2))
-
-          (ensures eq (do (v_of s2') last2) (concrete_merge (v_of lca) (v_of s1) (do (v_of s2') last2))) = ()
-          
-#push-options "--z3rlimit 200"
-let linearizable_s1_0''_merge_pre (lca s1 s2':st) (last2:op_t)
-  : Lemma (requires do_pre (v_of s2') last2 /\
-                    consistent_branches lca s1 (do_st s2' last2) /\
-                    ops_of s1 = ops_of lca /\
-                    length (ops_of s2') > length (ops_of lca) /\
-
-                    (let inv2 = inverse_st s2' in
-                    do_pre (v_of inv2) last2 /\
-                    consistent_branches lca s1 (do_st inv2 last2) /\
-                    merge_pre (v_of lca) (v_of s1) (do (v_of s2') last2)))
-         
-          (ensures merge_pre (v_of lca) (v_of s1) (do (v_of (inverse_st s2')) last2)) = ()
-
-let linearizable_s1_0''_ind (lca s1 s2':st) (last2:op_t)
-  : Lemma (requires do_pre (v_of s2') last2 /\
-                    consistent_branches lca s1 (do_st s2' last2) /\
-                    ops_of s1 = ops_of lca /\
-                    length (ops_of s2') > length (ops_of lca) /\
-
-                    (let inv2 = inverse_st s2' in
-                    do_pre (v_of inv2) last2 /\
-                    consistent_branches lca s1 (do_st inv2 last2) /\
-                    merge_pre (v_of lca) (v_of s1) (do (v_of inv2) last2) /\
-                    eq (do (v_of inv2) last2) (concrete_merge (v_of lca) (v_of s1) (do (v_of inv2) last2))) /\
-                    merge_pre (v_of lca) (v_of s1) (do (v_of s2') last2))
-        
-          (ensures eq (do (v_of s2') last2) (concrete_merge (v_of lca) (v_of s1) (do (v_of s2') last2))) = ()
-
-let linearizable_s1_0_s2_0_base (lca s1 s2:st)
+let linearizable_s1_0' (lca s1 s2:st)
   : Lemma (requires consistent_branches lca s1 s2 /\
-                    ops_of s1 == ops_of lca /\ ops_of s2 == ops_of lca /\
+                    ops_of s1 = ops_of lca /\
                     merge_pre (v_of lca) (v_of s1) (v_of s2))
-        
-          (ensures eq (v_of lca) (concrete_merge (v_of lca) (v_of s1) (v_of s2))) = ()
+          (ensures eq (v_of s2) (concrete_merge (v_of lca) (v_of s1) (v_of s2))) = ()
 
-let linearizable_gt0_base_fts (lca s1 s2:st) (last1 last2:op_t)
+let linearizable_s2_0' (lca s1 s2:st)
+  : Lemma (requires consistent_branches lca s1 s2 /\
+                    ops_of s2 = ops_of lca /\
+                    merge_pre (v_of lca) (v_of s1) (v_of s2))
+          (ensures eq (v_of s1) (concrete_merge (v_of lca) (v_of s1) (v_of s2))) = ()
+
+let pre1_pre2_s2 (lca s1 s2:st)
+    : Lemma (requires consistent_branches_s2_gt0 lca s1 s2)
+            (ensures consistent_branches lca s1 (inverse_st s2)) = 
+  lem_inverse (ops_of lca) (ops_of s2);
+  lastop_diff (ops_of lca) (ops_of s2);
+  inverse_diff_id_s2' (ops_of lca) (ops_of s1) (ops_of s2)
+
+let pre1_pre2_s1 (lca s1 s2:st)
+    : Lemma (requires consistent_branches_s1_gt0 lca s1 s2)
+            (ensures consistent_branches lca (inverse_st s1) s2) = 
+  lem_inverse (ops_of lca) (ops_of s1);
+  lastop_diff (ops_of lca) (ops_of s1);
+  inverse_diff_id_s1' (ops_of lca) (ops_of s1) (ops_of s2)
+  
+#push-options "--z3rlimit 600" 
+let rec invalid_exec1 (lca s1 s2:st) (last1 last2:op_t)
   : Lemma (requires do_pre (v_of s1) last1 /\ do_pre (v_of s2) last2 /\ 
                     consistent_branches lca (do_st s1 last1) (do_st s2 last2) /\
                     consistent_branches lca s1 s2 /\
-                    ops_of s1 = ops_of lca /\ ops_of s2 = ops_of lca /\
+                    Add_after? (snd last1) /\ Remove? (snd last2) /\
+                    fst last1 <> fst last2)
+          (ensures (fst last1 <> get_rem_id last2) (*/\
+                   (Remove? (snd last1) /\ Add_after? (snd last2) ==> fst last2 <> get_rem_id last1) /\
+                   (Add_after? (snd last1) /\ Add_after? (snd last2) ==>
+                      fst last1 <> get_after_id last2 /\ fst last2 <> get_after_id last1*))
+          (decreases %[length (ops_of s1); length (ops_of s2)]) = 
+  //assume ((fst last1 = get_rem_id last2) ==> ~ (Add_after? (snd last1) /\ Remove? (snd last2)));
+  if ops_of lca = ops_of s1 then
+    (if ops_of lca = ops_of s2 then admit()
+     else 
+       (let s2' = inverse_st s2 in
+        let pre2, lastop2 = un_snoc (ops_of s2) in
+        do_prop (v_of s2') last2; //include it if needed
+        lem_apply_log init_st (ops_of s2);
+        inverse_helper init_st pre2 lastop2;
+        assume (mem_id_s (get_rem_id last2) (fst (v_of s2')) <==> do_pre (v_of s2') last2);
+        pre1_pre2_s2 lca s1 s2;
+        if mem_id_s (get_rem_id last2) (fst (v_of s2')) then 
+          (admit();assume (do_pre (v_of s2') last2); 
+           assume (consistent_branches lca (do_st s1 last1) (do_st s2' last2)); //can be done
+           invalid_exec1 lca s1 s2' last1 last2)
+        else 
+          (assume (not (mem_id_s (get_rem_id last2) (fst (v_of s2'))));
+           if Add_after? (snd lastop2) && fst lastop2 = get_rem_id last2 then 
+             (lem_diff (snoc (ops_of s2) last2) (ops_of lca);
+              lem_diff (ops_of s2) (ops_of lca); 
+              assume (mem_id (fst lastop2) (diff (ops_of s2) (ops_of lca)));
+              assume (not (mem_id (fst lastop2) (ops_of lca)));
+              assume (mem_id (fst lastop2) (ops_of s2));
+              lemma_append_count_assoc_fst (ops_of s2) (create 1 last2);
+              assume (mem_id (fst lastop2) (snoc (ops_of s2) last2)); 
+              lemma_append_count_assoc_fst (snoc (ops_of s2) last2) (create 1 last2);
+              assume (mem_id (fst lastop2) (diff (snoc (ops_of s2) last2) (ops_of lca)));
+              lem_diff (snoc (ops_of s1) last1) (ops_of lca);
+              assume (mem_id (fst last1) (diff (snoc (ops_of s1) last1) (ops_of lca))); //done
+              ()) 
+           else 
+             (admit();assume (do_pre (v_of s2') last2); 
+              assume (consistent_branches lca (do_st s1 last1) (do_st s2' last2)); //can be done
+              invalid_exec1 lca s1 s2' last1 last2))))
+  else 
+    (admit()(*;let s1' = inverse_st s1 in 
+     assume (consistent_branches_s1_gt0 lca s1 s2);
+     let pre1, lastop1 = un_snoc (ops_of s1) in
+     do_prop (v_of s1') last1; //include it if needed
+     lem_apply_log init_st (ops_of s1);
+     inverse_helper init_st pre1 lastop1;
+     pre1_pre2_s1 lca s1 s2;
+     assume (fst lastop1 <> fst last1); //can be done
+     if Add_after? (snd lastop1) && fst lastop1 <> get_after_id last1 then 
+       (admit();assume (not (mem_id_s (fst last1) (fst (v_of s1'))));
+        //assume (~ (get_after_id last1 = 0) ==> mem_id_s (get_after_id last1) (fst (v_of s1')));
+        assume (do_pre (v_of s1') last1);
+        assume (consistent_branches lca (do_st s1' last1) (do_st s2 last2)); //can be done
+        invalid_exec1 lca s1' s2 last1 last2)
+     else if Add_after? (snd lastop1) && fst lastop1 = get_after_id last1 then  //check this case with full do_pre for add
+       (admit();assume (not (mem_id_s (fst last1) (fst (v_of s1')))); 
+        //assert (~ (get_after_id last1 = 0) ==> mem_id_s (get_after_id last1) (fst (v_of s1')));
+        assume (do_pre (v_of s1') last1);
+        assume (consistent_branches lca (do_st s1' last1) (do_st s2 last2)); //can be done
+        invalid_exec1 lca s1' s2 last1 last2)
+     else if Remove? (snd lastop1) && get_rem_id lastop1 <> fst last1 then
+       (admit();assume (do_pre (v_of s1') last1); 
+        assume (consistent_branches lca (do_st s1' last1) (do_st s2 last2)); //can be done
+        invalid_exec1 lca s1' s2 last1 last2)
+     else admit()*)) //Remove? (snd lastop1) && get_rem_id lastop1 = fst last1
+
+let rec invalid_exec (lca s1 s2:st) (last1 last2:op_t)
+  : Lemma (requires do_pre (v_of s1) last1 /\ do_pre (v_of s2) last2 /\ 
+                    consistent_branches lca (do_st s1 last1) (do_st s2 last2) /\
+                    consistent_branches lca s1 s2 /\
+                    fst last1 <> fst last2)
+          (ensures (Remove? (snd last1) /\ Add_after? (snd last2) ==> fst last2 <> get_rem_id last1) /\
+                   (Remove? (snd last2) /\ Add_after? (snd last1) ==> fst last1 <> get_rem_id last2) /\
+                   (Add_after? (snd last1) /\ Add_after? (snd last2) ==>
+                      fst last1 <> get_after_id last2 /\ fst last2 <> get_after_id last1)) = 
+  if Add_after? (snd last1) && Remove? (snd last2) then
+    invalid_exec1 lca s1 s2 last1 last2
+  else 
+    (assume ((Remove? (snd last1) /\ Add_after? (snd last2) ==> fst last2 <> get_rem_id last1) /\
+             (Add_after? (snd last1) /\ Add_after? (snd last2) ==>
+                      fst last1 <> get_after_id last2 /\ fst last2 <> get_after_id last1));
+     ())
+  
+
+#push-options "--z3rlimit 100" //with subset pre
+let linearizable_gt0_s1' (lca s1 s2:st) (last1 last2:op_t)
+  : Lemma (requires do_pre (v_of s1) last1 /\ do_pre (v_of s2) last2 /\ 
+                    consistent_branches lca (do_st s1 last1) (do_st s2 last2) /\
+                    consistent_branches lca s1 (do_st s2 last2) /\
+                    consistent_branches lca s1 s2 /\
+                    is_prefix (ops_of lca) (ops_of s2) /\
                     fst last1 <> fst last2 /\
-                    merge_pre (v_of lca) (do (v_of s1) last1) (do (v_of s2) last2) /\
-                    First_then_second? (resolve_conflict last1 last2))
-         
-          (ensures merge_pre (v_of lca) (v_of s1) (do (v_of s2) last2) /\
-                   do_pre (concrete_merge (v_of lca) (v_of s1) (do (v_of s2) last2)) last1 /\
+                    First_then_second? (resolve_conflict last1 last2) /\
+                    //Remove? (snd last1) /\ Remove? (snd last2) /\ //all done
+                    //Add_after? (snd last1) /\ Remove? (snd last2) /\
+                    //Add_after? (snd last1) /\ Add_after? (snd last2) /\ get_after_id last1 <> get_after_id last2 /\
+                    //Add_after? (snd last1) /\ Add_after? (snd last2) /\ get_after_id last1 = get_after_id last2 /\ fst last1 > fst last2 /\
+                    merge_pre (v_of lca) (do (v_of s1) last1) (do (v_of s2) last2))
+          (ensures merge_pre (v_of lca) (v_of s1) (do (v_of s2) last2) /\ //only w/o subset pre
+                   do_pre (concrete_merge (v_of lca) (v_of s1) (do (v_of s2) last2)) last1 /\ //only with subset pre
                    eq (do (concrete_merge (v_of lca) (v_of s1) (do (v_of s2) last2)) last1)
                       (concrete_merge (v_of lca) (do (v_of s1) last1) (do (v_of s2) last2))) = 
-  assume (//(Remove? (snd last1) /\ Add_after? (snd last2) ==> fst last2 <> get_rem_id last1) /\
+  invalid_exec lca s1 s2 last1 last2
+
+let linearizable_gt0_s2' (lca s1 s2:st) (last1 last2:op_t)
+  : Lemma (requires do_pre (v_of s1) last1 /\ do_pre (v_of s2) last2 /\ 
+                    consistent_branches lca (do_st s1 last1) (do_st s2 last2) /\
+                    //consistent_branches lca (do_st s1 last1) s2 /\
+                    consistent_branches lca s1 s2 /\
+                    //is_prefix (ops_of lca) (ops_of s1) /\
+                    fst last1 <> fst last2 /\
+                    //Second_then_first? (resolve_conflict last1 last2) /\
+                    Remove? (snd last1) /\ Add_after? (snd last2) /\
+  //                  Add_after? (snd last1) /\ Add_after? (snd last2) /\ get_after_id last1 = get_after_id last2 /\ fst last1 < fst last2 /\
+                    merge_pre (v_of lca) (do (v_of s1) last1) (do (v_of s2) last2) /\
+                    merge_pre (v_of lca) (do (v_of s1) last1) (v_of s2))
+                    //do_pre (concrete_merge (v_of lca) (do (v_of s1) last1) (v_of s2)) last2) 
+          (ensures //merge_pre (v_of lca) (do (v_of s1) last1) (v_of s2) /\
+                   do_pre (concrete_merge (v_of lca) (do (v_of s1) last1) (v_of s2)) last2 (*/\
+                   eq (do (concrete_merge (v_of lca) (do (v_of s1) last1) (v_of s2)) last2)
+                      (concrete_merge (v_of lca) (do (v_of s1) last1) (do (v_of s2) last2)*)) =
+  //invalid_exec lca s1 s2 last1 last2;
+  assert ((Remove? (snd last1) /\ Add_after? (snd last2) ==> fst last2 <> get_rem_id last1) /\
           (Add_after? (snd last1) /\ Add_after? (snd last2) ==>
-                      fst last1 <> get_after_id last2 /\ fst last2 <> get_after_id last1)); //used for eq
-  ()
-
-let linearizable_gt0_base_stf (lca s1 s2:st) (last1 last2:op_t)
-  : Lemma (requires do_pre (v_of s1) last1 /\ do_pre (v_of s2) last2 /\ 
-                    consistent_branches lca (do_st s1 last1) (do_st s2 last2) /\
-                    consistent_branches lca s1 s2 /\
-                    ops_of s1 = ops_of lca /\ ops_of s2 = ops_of lca /\
-                    fst last1 <> fst last2 /\
-                    merge_pre (v_of lca) (do (v_of s1) last1) (do (v_of s2) last2) /\
-                    Second_then_first? (resolve_conflict last1 last2))
-         
-          (ensures merge_pre (v_of lca) (do (v_of s1) last1) (v_of s2) /\
-                   do_pre (concrete_merge (v_of lca) (do (v_of s1) last1) (v_of s2)) last2 /\
-                   eq (do (concrete_merge (v_of lca) (do (v_of s1) last1) (v_of s2)) last2)
-                      (concrete_merge (v_of lca) (do (v_of s1) last1) (do (v_of s2) last2))) = ()
-
-let linearizable_gt0_base (lca s1 s2:st) (last1 last2:op_t)
-  : Lemma (requires do_pre (v_of s1) last1 /\ do_pre (v_of s2) last2 /\ 
-                    consistent_branches lca (do_st s1 last1) (do_st s2 last2) /\
-                    consistent_branches lca s1 s2 /\
-                    ops_of s1 = ops_of lca /\ ops_of s2 = ops_of lca /\
-                    fst last1 <> fst last2 /\
-                    merge_pre (v_of lca) (do (v_of s1) last1) (do (v_of s2) last2))
-         
-          (ensures (First_then_second? (resolve_conflict last1 last2) ==>
-                      merge_pre (v_of lca) (v_of s1) (do (v_of s2) last2) /\
-                      do_pre (concrete_merge (v_of lca) (v_of s1) (do (v_of s2) last2)) last1 /\
-                      (eq (do (concrete_merge (v_of lca) (v_of s1) (do (v_of s2) last2)) last1)
-                          (concrete_merge (v_of lca) (do (v_of s1) last1) (do (v_of s2) last2)))) /\
-
-                   (Second_then_first? (resolve_conflict last1 last2) ==>
-                      merge_pre (v_of lca) (do (v_of s1) last1) (v_of s2) /\
-                      do_pre (concrete_merge (v_of lca) (do (v_of s1) last1) (v_of s2)) last2 /\
-                      (eq (do (concrete_merge (v_of lca) (do (v_of s1) last1) (v_of s2)) last2)
-                          (concrete_merge (v_of lca) (do (v_of s1) last1) (do (v_of s2) last2))))) =
-  if First_then_second? (resolve_conflict last1 last2) then
-    linearizable_gt0_base_fts lca s1 s2 last1 last2
-  else if Second_then_first? (resolve_conflict last1 last2) then
-    linearizable_gt0_base_stf lca s1 s2 last1 last2
-  else ()
-
-let linearizable_gt0_s2'_do_pre (lca s1 s2:st) (last1 last2:op_t)
-  : Lemma (requires do_pre (v_of s1) last1 /\ do_pre (v_of s2) last2 /\ 
-                    consistent_branches lca (do_st s1 last1) (do_st s2 last2) /\
-                    consistent_branches lca (do_st s1 last1) s2 /\
-                    consistent_branches lca s1 s2 /\
-                    fst last1 <> fst last2 /\
-                    Second_then_first? (resolve_conflict last1 last2)) 
-         
-          (ensures (length (ops_of s2) > length (ops_of lca) ==> do_pre (v_of (inverse_st s2)) last2) /\
-                   (length (ops_of s1) > length (ops_of lca) ==> do_pre (v_of (inverse_st s1)) last1)) = ()
-
-let linearizable_gt0_s2'_merge_pre (lca s1 s2:st) (last1 last2:op_t)
-  : Lemma (requires do_pre (v_of s1) last1 /\ do_pre (v_of s2) last2 /\ 
-                    consistent_branches lca (do_st s1 last1) (do_st s2 last2) /\
-                    consistent_branches lca (do_st s1 last1) s2 /\
-                    consistent_branches lca s1 s2 /\
-                    fst last1 <> fst last2 /\
-                    Second_then_first? (resolve_conflict last1 last2) /\
-                    merge_pre (v_of lca) (do (v_of s1) last1) (do (v_of s2) last2))
-         
-          (ensures (length (ops_of s1) > length (ops_of lca) /\ do_pre (v_of (inverse_st s1)) last1 ==>
-                      merge_pre (v_of lca) (do (v_of (inverse_st s1)) last1) (do (v_of s2) last2)) /\
-                   (length (ops_of s2) > length (ops_of lca) /\ do_pre (v_of (inverse_st s2)) last2 ==>
-                      merge_pre (v_of lca) (do (v_of s1) last1) (do (v_of (inverse_st s2)) last2))) = ()
-                      
-let linearizable_gt0_s1'_do_pre (lca s1 s2:st) (last1 last2:op_t)
-  : Lemma (requires do_pre (v_of s1) last1 /\ do_pre (v_of s2) last2 /\ 
-                    consistent_branches lca (do_st s1 last1) (do_st s2 last2) /\
-                    consistent_branches lca s1 (do_st s2 last2) /\
-                    consistent_branches lca s1 s2 /\
-                    fst last1 <> fst last2 /\
-                    First_then_second? (resolve_conflict last1 last2)) 
-          (ensures (length (ops_of s2) > length (ops_of lca) ==> do_pre (v_of (inverse_st s2)) last2) /\
-                   (length (ops_of s1) > length (ops_of lca) ==> do_pre (v_of (inverse_st s1)) last1)) = ()
-
-let linearizable_gt0_s1'_merge_pre (lca s1 s2:st) (last1 last2:op_t)
-  : Lemma (requires do_pre (v_of s1) last1 /\ do_pre (v_of s2) last2 /\ 
-                    consistent_branches lca (do_st s1 last1) (do_st s2 last2) /\
-                    consistent_branches lca s1 (do_st s2 last2) /\
-                    consistent_branches lca s1 s2 /\
-                    fst last1 <> fst last2 /\
-                    First_then_second? (resolve_conflict last1 last2) /\
-                    merge_pre (v_of lca) (do (v_of s1) last1) (do (v_of s2) last2))
-          (ensures (length (ops_of s1) > length (ops_of lca) /\ do_pre (v_of (inverse_st s1)) last1 ==>
-                      merge_pre (v_of lca) (do (v_of (inverse_st s1)) last1) (do (v_of s2) last2)) /\
-                   (length (ops_of s2) > length (ops_of lca) /\ do_pre (v_of (inverse_st s2)) last2 ==>
-                      merge_pre (v_of lca) (do (v_of s1) last1) (do (v_of (inverse_st s2)) last2))) = ()
-
-#push-options "--z3rlimit 600"
-let linearizable_gt0_ind_fts (lca s1 s2:st) (last1 last2:op_t)
-  : Lemma (requires do_pre (v_of s1) last1 /\ do_pre (v_of s2) last2 /\ 
-                    //consistent_branches lca (do_st s1 last1) (do_st s2 last2) /\
-                    //consistent_branches lca s1 s2 /\
-                    length (ops_of s2) > length (ops_of lca) /\
-                    fst last1 <> fst last2 /\
-                    merge_pre (v_of lca) (do (v_of s1) last1) (do (v_of s2) last2) /\
-                    (let s2' = inverse_st s2 in
-                    do_pre (v_of s2') last2 /\
-                    First_then_second? (resolve_conflict last1 last2) /\
-                    //Remove? (snd last1) /\ Remove? (snd last2) /\ //all done
-                    //Add_after? (snd last1) /\ Remove? (snd last2) /\
-                    //Add_after? (snd last1) /\ Add_after? (snd last2) /\ get_after_id last1 <> get_after_id last2 /\
-                    //Add_after? (snd last1) /\ Add_after? (snd last2) /\ get_after_id last1 = get_after_id last2 /\ fst last1 > fst last2 /\
-                    //consistent_branches lca s1 (do_st s2' last2) /\
-                    //consistent_branches lca (do_st s1 last1) (do_st s2' last2) /\
-                    //consistent_branches lca s1 (do_st s2 last2) /\
-                    merge_pre (v_of lca) (v_of s1) (do (v_of s2') last2) /\
-                    merge_pre (v_of lca) (do (v_of s1) last1) (do (v_of s2') last2) /\
-                    do_pre (concrete_merge (v_of lca) (v_of s1) (do (v_of s2') last2)) last1 /\
-                    eq (do (concrete_merge (v_of lca) (v_of s1) (do (v_of s2') last2)) last1)
-                       (concrete_merge (v_of lca) (do (v_of s1) last1) (do (v_of s2') last2))))
-       
-          (ensures merge_pre (v_of lca) (v_of s1) (do (v_of s2) last2) /\
-                   do_pre (concrete_merge (v_of lca) (v_of s1) (do (v_of s2) last2)) last1 /\
-                   eq (do (concrete_merge (v_of lca) (v_of s1) (do (v_of s2) last2)) last1)
-                        (concrete_merge (v_of lca) (do (v_of s1) last1) (do (v_of s2) last2))) = 
-  
-  lem_apply_log init_st (ops_of s2);
-  let pre, lastop = un_snoc (ops_of s2) in
-  inverse_helper init_st pre lastop;
-  assume (Remove? (snd last1) ==> get_rem_id last1 <> fst lastop);
-  assume (Add_after? (snd last1) /\ Remove? (snd last2) ==> fst last1 <> get_rem_id last2 /\ fst last1 <> fst lastop); 
-  assume (Add_after? (snd last1) /\ Remove? (snd last2) /\ Remove? (snd lastop) ==> fst last1 <> get_rem_id lastop);
-  assume (Add_after? (snd last1) /\ Remove? (snd last2) /\ Add_after? (snd lastop) ==>
-                fst last1 <> get_after_id lastop /\ fst lastop <> get_after_id last1); 
-  assume ((Add_after? (snd last1) /\ Add_after? (snd last2) ==> fst last1 <> fst lastop /\
-                      fst last1 <> get_after_id last2 /\ fst last2 <> get_after_id last1)); 
-  assume (Add_after? (snd last1) /\ Add_after? (snd last2) /\ Add_after? (snd lastop) ==>
-                     fst last1 <> get_after_id lastop /\ fst lastop <> get_after_id last1); 
-  assume (Add_after? (snd last1) /\ Add_after? (snd last2) /\ Remove? (snd lastop) ==>
-                     fst last1 <> get_rem_id lastop);
-  ()
- 
-let linearizable_gt0_ind_stf (lca s1 s2:st) (last1 last2:op_t)
-  : Lemma (requires do_pre (v_of s1) last1 /\ do_pre (v_of s2) last2 /\ 
-                    //consistent_branches lca (do_st s1 last1) (do_st s2 last2) /\
-                    //consistent_branches lca s1 s2 /\
-                    length (ops_of s2) > length (ops_of lca) /\
-                    fst last1 <> fst last2 /\
-                    merge_pre (v_of lca) (do (v_of s1) last1) (do (v_of s2) last2) /\
-                    (let s2' = inverse_st s2 in
-                    do_pre (v_of s2') last2 /\
-                    ops_of s1 = ops_of lca /\
-                    Second_then_first? (resolve_conflict last1 last2) /\
-                    //Remove? (snd last1) /\ Add_after? (snd last2) /\
-                    //Add_after? (snd last1) /\ Add_after? (snd last2) /\ get_after_id last1 = get_after_id last2 /\ fst last1 < fst last2 /\
-                    //consistent_branches lca (do_st s1 last1) s2' /\
-                    //consistent_branches lca (do_st s1 last1) (do_st s2' last2) /\
-                    //consistent_branches lca (do_st s1 last1) s2 /\
-                    merge_pre (v_of lca) (do (v_of s1) last1) (v_of s2') /\
-                    do_pre (concrete_merge (v_of lca) (do (v_of s1) last1) (v_of s2')) last2 /\
-                    merge_pre (v_of lca) (do (v_of s1) last1) (do (v_of s2') last2) /\
-                    eq (do (concrete_merge (v_of lca) (do (v_of s1) last1) (v_of s2')) last2)
-                       (concrete_merge (v_of lca) (do (v_of s1) last1) (do (v_of s2') last2))))
-       
-          (ensures merge_pre (v_of lca) (do (v_of s1) last1) (v_of s2) /\
-                   do_pre (concrete_merge (v_of lca) (do (v_of s1) last1) (v_of s2)) last2 /\
-                   eq (do (concrete_merge (v_of lca) (do (v_of s1) last1) (v_of s2)) last2)
-                      (concrete_merge (v_of lca) (do (v_of s1) last1) (do (v_of s2) last2))) 
-          (*[SMTPat (eq (do (concrete_merge (v_of lca) (do (v_of s1) last1) (v_of s2)) last2)
-                      (concrete_merge (v_of lca) (do (v_of s1) last1) (do (v_of s2) last2)))]*) = ()
-
-let linearizable_gt0_ind1_fts (lca s1 s2:st) (last1 last2:op_t)
-  : Lemma (requires do_pre (v_of s1) last1 /\ do_pre (v_of s2) last2 /\ 
-                    //consistent_branches lca (do_st s1 last1) (do_st s2 last2) /\
-                    //consistent_branches lca s1 s2 /\
-                    length (ops_of s1) > length (ops_of lca) /\
-                    fst last1 <> fst last2 /\
-                    merge_pre (v_of lca) (do (v_of s1) last1) (do (v_of s2) last2) /\
-                    (let s1' = inverse_st s1 in
-                    do_pre (v_of s1') last1 /\
-                    ops_of s2 = ops_of lca /\
-                    First_then_second? (resolve_conflict last1 last2) /\
-                    //Remove? (snd last1) /\ Remove? (snd last2) /\ //all done
-                    //Add_after? (snd last1) /\ Remove? (snd last2) /\
-                    //Add_after? (snd last1) /\ Add_after? (snd last2) /\ get_after_id last1 <> get_after_id last2 /\
-                    //Add_after? (snd last1) /\ Add_after? (snd last2) /\ get_after_id last1 = get_after_id last2 /\ fst last1 > fst last2 /\
-                    //consistent_branches lca s1' (do_st s2 last2) /\
-                    //consistent_branches lca (do_st s1' last1) (do_st s2 last2) /\
-                    //consistent_branches lca s1 (do_st s2 last2) /\
-                    merge_pre (v_of lca) (v_of s1') (do (v_of s2) last2) /\
-                    merge_pre (v_of lca) (do (v_of s1') last1) (do (v_of s2) last2) /\
-                    do_pre (concrete_merge (v_of lca) (v_of s1') (do (v_of s2) last2)) last1 /\
-                    eq (do (concrete_merge (v_of lca) (v_of s1') (do (v_of s2) last2)) last1)
-                       (concrete_merge (v_of lca) (do (v_of s1') last1) (do (v_of s2) last2))))
-                    
-          (ensures merge_pre (v_of lca) (v_of s1) (do (v_of s2) last2) /\
-                   do_pre (concrete_merge (v_of lca) (v_of s1) (do (v_of s2) last2)) last1 /\
-                   eq (do (concrete_merge (v_of lca) (v_of s1) (do (v_of s2) last2)) last1)
-                      (concrete_merge (v_of lca) (do (v_of s1) last1) (do (v_of s2) last2))) = ()
-
-let linearizable_gt0_ind1_stf (lca s1 s2:st) (last1 last2:op_t)
-  : Lemma (requires do_pre (v_of s1) last1 /\ do_pre (v_of s2) last2 /\ 
-                    //consistent_branches lca (do_st s1 last1) (do_st s2 last2) /\
-                    //consistent_branches lca s1 s2 /\
-                    length (ops_of s1) > length (ops_of lca) /\
-                    fst last1 <> fst last2 /\
-                    merge_pre (v_of lca) (do (v_of s1) last1) (do (v_of s2) last2) /\
-                    (let s1' = inverse_st s1 in
-                    do_pre (v_of s1') last1 /\
-                    Second_then_first? (resolve_conflict last1 last2) /\
-                    //Remove? (snd last1) /\ Add_after? (snd last2) /\
-                    //Add_after? (snd last1) /\ Add_after? (snd last2) /\ get_after_id last1 = get_after_id last2 /\ fst last1 < fst last2 /\
-                    //consistent_branches lca (do_st s1' last1) s2 /\
-                    //consistent_branches lca (do_st s1' last1) (do_st s2 last2) /\
-                    //consistent_branches lca (do_st s1 last1) s2 /\
-                    merge_pre (v_of lca) (do (v_of s1') last1) (v_of s2) /\
-                    merge_pre (v_of lca) (do (v_of s1') last1) (do (v_of s2) last2) /\
-                    do_pre (concrete_merge (v_of lca) (do (v_of s1') last1) (v_of s2)) last2 /\
-                    eq (do (concrete_merge (v_of lca) (do (v_of s1') last1) (v_of s2)) last2)
-                       (concrete_merge (v_of lca) (do (v_of s1') last1) (do (v_of s2) last2))))
-                           
-          (ensures merge_pre (v_of lca) (do (v_of s1) last1) (v_of s2) /\
-                   do_pre (concrete_merge (v_of lca) (do (v_of s1) last1) (v_of s2)) last2 /\    
-                   eq (do (concrete_merge (v_of lca) (do (v_of s1) last1) (v_of s2)) last2)
-                      (concrete_merge (v_of lca) (do (v_of s1) last1) (do (v_of s2) last2))) =  //both do_pre and eq
-  
-  lem_apply_log init_st (ops_of s1);
-  let pre, lastop = un_snoc (ops_of s1) in
-  inverse_helper init_st pre lastop;
-  assume (Remove? (snd last1) /\ Add_after? (snd last2) ==> fst last2 <> get_rem_id last1 /\ fst last2 <> fst lastop);
-  assume (Remove? (snd last1) /\ Add_after? (snd last2) /\ Remove? (snd lastop) ==> fst last2 <> get_rem_id lastop);
-  assume (Remove? (snd last1) /\ Add_after? (snd last2) /\ Add_after? (snd lastop) ==>
-                fst last2 <> get_after_id lastop /\ fst lastop <> get_after_id last2);
-  assume ((Add_after? (snd last1) /\ Add_after? (snd last2) ==> fst last2 <> fst lastop /\
                       fst last1 <> get_after_id last2 /\ fst last2 <> get_after_id last1));
-  assume (Add_after? (snd last1) /\ Add_after? (snd last2) /\ Add_after? (snd lastop) ==>
-                     fst last2 <> get_after_id lastop /\ fst lastop <> get_after_id last2);
-  assume (Add_after? (snd last1) /\ Add_after? (snd last2) /\ Remove? (snd lastop) ==>
-                     fst last2 <> get_rem_id lastop);
   ()
-
-let fts_merge_pre' (lca s1 s2:st)
-  : Lemma (requires consistent_branches lca s1 s2 /\
-                    merge_pre (v_of lca) (v_of s1) (v_of s2) /\
-                    length (ops_of s1) > length (ops_of lca) /\
-                    length (ops_of s2) > length (ops_of lca) /\
-                    (let _, last1 = un_snoc (ops_of s1) in
-                     let _, last2 = un_snoc (ops_of s2) in
-                     fst last1 <> fst last2 /\
-                     First_then_second? (resolve_conflict last1 last2)))
-          (ensures merge_pre (v_of lca) (v_of (inverse_st s1)) (v_of s2)) = ()
-
-let stf_merge_pre' (lca s1 s2:st)
-  : Lemma (requires consistent_branches lca s1 s2 /\
-                    merge_pre (v_of lca) (v_of s1) (v_of s2) /\
-                    length (ops_of s1) > length (ops_of lca) /\
-                    length (ops_of s2) > length (ops_of lca) /\
-                    (let _, last1 = un_snoc (ops_of s1) in
-                     let _, last2 = un_snoc (ops_of s2) in
-                     fst last1 <> fst last2 /\
-                     Second_then_first? (resolve_conflict last1 last2)))
-          (ensures merge_pre (v_of lca) (v_of s1) (v_of (inverse_st s2))) = ()
